src/POCS.v
@@ -26,6 +26,8 @@ infrastructure. *)
 
 Require Export Helpers.Helpers.
 Require Export Helpers.ListStuff.
+Require Export Helpers.Sets.
+Require Export Helpers.Ordering.
 
 Require Export Spec.ConcurProc.
 Require Export Spec.Equiv.
